Add eq, choice and ordType to queries

src/Query.v
@@ -23,6 +23,8 @@ Section Query.
 
   Variables Name Vals : ordType.
 
+  
+  Unset Elimination Schemes.
   Inductive QuerySet : Type :=
   | SingleQuery : Query -> QuerySet
   | SelectionSet : Query -> QuerySet -> QuerySet
@@ -34,7 +36,6 @@ Section Query.
        | InlineFragment : Name -> QuerySet -> Query.
 
 
-  Unset Elimination Schemes.
   Inductive Result : Type :=
   | Results : list ResponseObject -> Result
   with ResponseObject : Type :=
@@ -46,13 +47,111 @@ Section Query.
   
   Set Elimination Schemes.
 
+  Scheme QuerySet_ind := Induction for QuerySet Sort Prop
+    with Query_ind := Induction for Query Sort Prop.
 
   Coercion responses_of_result (result : Result) := let: Results rs := result in rs.
 
 
-  
-  
 
+
+
+
+
+  
+  Fixpoint tree_of_query_set query_set : GenTree.tree (Name * Name * {fmap Name -> Vals}) :=
+    match query_set with
+    | SingleQuery q => GenTree.Node 0 [:: tree_of_query q]
+    | SelectionSet q q' => GenTree.Node 1 [:: (tree_of_query q) ; (tree_of_query_set q')]
+    end
+  with tree_of_query query : GenTree.tree (Name * Name * {fmap Name -> Vals}) :=
+         match query with
+         | SingleField n args => GenTree.Node 2 [:: GenTree.Leaf (n, n, args)]
+         | LabeledField l n args => GenTree.Node 3 [:: GenTree.Leaf (l, n, args)]
+         | NestedField n args ϕ => GenTree.Node 4 [:: GenTree.Leaf (n, n, args) ; (tree_of_query_set ϕ)]
+         | NestedLabeledField l n args ϕ => GenTree.Node 5 [:: GenTree.Leaf (l, n, args) ; (tree_of_query_set ϕ)]
+         | InlineFragment t ϕ => GenTree.Node 6 [:: GenTree.Leaf (t, t, emptym) ; (tree_of_query_set ϕ)]
+         end.
+
+  Fixpoint query_set_of_tree tree : option QuerySet :=
+    match tree with
+    | GenTree.Node 0 [:: t] =>
+      if query_of_tree t is Some ϕ then
+        Some (SingleQuery ϕ)
+      else
+        None
+    | GenTree.Node 1 [:: t ; t'] =>
+      if (query_of_tree t, query_set_of_tree t') is (Some ϕ, Some ϕ') then
+        Some (SelectionSet ϕ ϕ')
+      else
+        None
+    | _ => None
+    end
+  with
+  query_of_tree tree : option Query :=
+    match tree with
+    | GenTree.Node 2 [:: GenTree.Leaf (_, n, args)] => Some (SingleField n args)
+    | GenTree.Node 3 [:: GenTree.Leaf (l, n, args)] => Some (LabeledField l n args)
+    | GenTree.Node 4 [:: GenTree.Leaf (_, n, args) ; t] =>
+      if (query_set_of_tree t) is Some ϕ then
+        Some (NestedField n args ϕ)
+      else
+        None
+    | GenTree.Node 5 [:: GenTree.Leaf (l, n, args) ; t] =>
+       if (query_set_of_tree t) is Some ϕ then
+        Some (NestedLabeledField l n args ϕ)
+      else
+        None
+    | GenTree.Node 6 [:: GenTree.Leaf (_, t, emptym) ; tree'] =>
+      if (query_set_of_tree tree') is Some ϕ then
+        Some (InlineFragment t ϕ)
+      else
+        None
+    | _ => None
+    end.
+
+
+  Lemma pcan_tree_of_query_set : pcancel tree_of_query_set query_set_of_tree.
+  Proof.
+    rewrite /pcancel => qs.    
+    elim qs using QuerySet_ind with (P0 := fun q : Query => query_of_tree (tree_of_query q) = Some q).
+      by move=> q /= ->.
+      by move=> q H q' Hq /=; rewrite H Hq.
+      by move=> *.
+      by move=> *.  
+      by move=> n args ϕ /= ->.
+      by move=> l n args ϕ /= ->.
+      by move=> t ϕ /= ->.
+  Qed.
+  Lemma pcan_tree_of_query : pcancel tree_of_query query_of_tree.
+  Proof.
+    move=> q; elim q using Query_ind with (P := fun qs => query_set_of_tree (tree_of_query_set qs) = Some qs).
+    by move=> *; apply pcan_tree_of_query_set.
+    by move=> *; apply pcan_tree_of_query_set.
+    by move=> *.
+    by move=> *.  
+    by move=> n args ϕ /= ->.
+    by move=> l n args ϕ /= ->.
+    by move=> t ϕ /= ->.
+  Qed.
+    
+    
+  Definition query_set_eqMixin := PcanEqMixin pcan_tree_of_query_set.
+  Canonical query_set_eqType := EqType QuerySet query_set_eqMixin.
+  Definition query_eqMixin := PcanEqMixin pcan_tree_of_query.
+  Canonical query_eqType := EqType Query query_eqMixin.
+
+  Definition query_set_choiceMixin := PcanChoiceMixin pcan_tree_of_query_set.
+  Canonical query_set_choiceType := ChoiceType QuerySet query_set_choiceMixin.
+  Definition query_choiceMixin := PcanChoiceMixin pcan_tree_of_query.
+  Canonical query_choiceType := ChoiceType Query query_choiceMixin.
+
+
+  Definition query_set_ordMixin := PcanOrdMixin pcan_tree_of_query_set.
+  Canonical query_set_ordType := OrdType QuerySet query_set_ordMixin.
+  Definition query_ordMixin := PcanOrdMixin pcan_tree_of_query.
+  Canonical query_ordType := OrdType Query query_ordMixin.
+  
   
 End Query.
 
